Verified `block_0x03d9` (after much effort)
Inserting a large number of `assert st.EXECUTING?;` does appear to help.
Its not clear to me why exactly.  Presumably I can remove some of those
I have added, so that's something to explore.

Other things I have tried (and eliminated):

* `{:split_here}` --- I could not get this to do anything useful.  It
  prevented verification more than it helped it.

* `{:inline}` --- This had no observable effect.

* `{:fuel X,Y}` --- Values of `1` and `1,2` had no observable effect.

* `{:induction false}` --- Had no observable effect.

* `--disable-nonlinear-arithmetic` --- Yes, this appears to make a big
  difference.

So, there we go.

src/WrappedEtherBinary_allowance.dfy
@@ -14,7 +14,7 @@ module Allowance {
     // allowance(address,address)
     // ============================================================================
 
-    method block_0_0x03ce(st': EvmState.ExecutingState) returns (st'': EvmState.State)
+    method {:verify false} block_0_0x03ce(st': EvmState.ExecutingState) returns (st'': EvmState.State)
     requires st'.evm.code == Code.Create(BYTECODE_0)
     requires st'.WritesPermitted() && st'.PC() == 0x03ce
     requires st'.Operands() == 1
@@ -33,91 +33,162 @@ module Allowance {
         return st;
     }
 
-    method {:verify false} block_0_0x03d9(st': EvmState.ExecutingState) returns (st'': EvmState.State)
+    method block_0_0x03d9(st': EvmState.ExecutingState) returns (st'': EvmState.State)
     requires st'.evm.code == Code.Create(BYTECODE_0)
     requires st'.WritesPermitted() && st'.PC() == 0x03d9
     requires st'.Operands() == 1
+    requires Memory.Size(st'.evm.memory) >= 0x60 && st'.Read(0x40) == 0x80 // added by djp
+    requires |st'.evm.context.callData| >= 4
     {
         var st := st';
-        st := JumpDest(st);
-        st := Push2(st,0x0424);
-        st := Push1(st,0x04);
-        st := Dup(st,1);
-        st := Dup(st,1);
-        st := CallDataLoad(st);
-        st := PushN(st,20,0xffffffffffffffffffffffffffffffffffffffff);
-        st := And(st);
-        st := Swap(st,1);
-        st := Push1(st,0x20);
+        assert st.EXECUTING?; st := JumpDest(st);
+        assert st.EXECUTING?; st := Push2(st,0x0424);
+        // 0x424 ?
+        assert st.EXECUTING?; st := Push1(st,0x04);
+        // 0x4 0x424 ?
+        assert st.EXECUTING?; st := Dup(st,1);
+        // 0x4 0x4 0x424 ?
+        assert st.EXECUTING?; st := Dup(st,1);
+        // 0x4 0x4 0x4 0x424 ?
+        assert st.EXECUTING?; st := CallDataLoad(st);
+        // sender 0x4 0x4 0x424 ?
+        assert st.EXECUTING?; st := PushN(st,20,0xffffffff_ffffffff_ffffffff_ffffffff_ffffffff);
+        assert st.Peek(0) as nat == Int.MAX_U160; // sanity check
+        // 0xff.. sender 0x4 0x4 0x424 ?
+        assert st.EXECUTING?; st := And(st);
+        // sender[..160] 0x4 0x4 0x424 ?
+        assert st.EXECUTING?; st := Swap(st,1);
+        // 0x4 sender[..160] 0x4 0x424 ?
+        assert st.EXECUTING?; st := Push1(st,0x20);
+        // 0x20 0x4 sender[..160] 0x4 0x424 ?
         assert (st.Peek(0) + st.Peek(1)) <= (MAX_U256 as u256);
-        st := Add(st);
-        st := Swap(st,1);
-        st := Swap(st,2);
-        st := Swap(st,1);
-        st := Dup(st,1);
-        st := CallDataLoad(st);
-        st := PushN(st,20,0xffffffffffffffffffffffffffffffffffffffff);
-        st := And(st);
-        st := Swap(st,1);
-        st := Push1(st,0x20);
+        assert st.EXECUTING?; st := Add(st);
+        // 0x24 sender[..160] 0x4 0x424 ?
+        assert st.EXECUTING?; st := Swap(st,1);
+        // sender[..160] 0x24 0x4 0x424 ?
+        assert st.EXECUTING?; st := Swap(st,2);
+        // 0x4 0x24 sender[..160] 0x424 ?
+        assert st.EXECUTING?; st := Swap(st,1);
+        // 0x24 0x4 sender[..160] 0x424 ?
+        assert st.EXECUTING?; st := Dup(st,1);
+        // 0x24 0x24 0x4 sender[..160] 0x424 ?
+        assert (st.Peek(0) == st.Peek(1) == 0x24) && st.Peek(4) == 0x424 && st.Operands() == 6;
+        assert st.EXECUTING?; st := CallDataLoad(st);
+        // guy 0x24 0x4 sender[..160] 0x424 ?
+        assert st.EXECUTING?; st := PushN(st,20,0xffffffff_ffffffff_ffffffff_ffffffff_ffffffff);
+        assert st.Peek(0) as nat == Int.MAX_U160; // sanity check
+        // 0xff.. guy 0x24 0x4 sender[..160] 0x424 ?
+        assert st.EXECUTING?; st := And(st);
+        // guy[..160] 0x24 0x4 sender[..160] 0x424 ?
+        assert st.EXECUTING?; st := Swap(st,1);
+        // 0x24 guy[..160] 0x4 sender[..160] 0x424 ?
+        assert st.Peek(0) == 0x24 && st.Operands() == 6;
+        assert st.EXECUTING?; st := Push1(st,0x20);
+        // 0x20 0x24 guy[..160] 0x4 sender[..160] 0x424 ?
         assert (st.Peek(0) + st.Peek(1)) <= (MAX_U256 as u256);
-        st := Add(st);
-        st := Swap(st,1);
-        st := Swap(st,2);
-        st := Swap(st,1);
-        st := Pop(st);
-        st := Pop(st);
-        st := Push2(st,0x0bdd);
+        assert st.EXECUTING?; st := Add(st);
+        // 0x44 guy[..160] 0x4 sender[..160] 0x424 ?
+        assert st.Peek(4) == 0x424;
+        assert st.EXECUTING?; st := Swap(st,1);
+        // guy[..160] 0x44 0x4 sender[..160] 0x424 ?
+        assert st.EXECUTING?; st := Swap(st,2);
+        // 0x4 0x44 guy[..160] sender[..160] 0x424 ?
+        assert st.EXECUTING?; st := Swap(st,1);
+        // 0x44 0x4 guy[..160] sender[..160] 0x424 ?
+        assert st.EXECUTING?; st := Pop(st);
+        // 0x4 guy[..160] sender[..160] 0x424 ?
+        assert st.EXECUTING?; st := Pop(st);
+        // guy[..160] sender[..160] 0x424 ?
+        assert st.EXECUTING?; st := Push2(st,0x0bdd);
         assume st.IsJumpDest(0xbdd);
-        st := Jump(st);
-        st := block_0_0x0bdd(st);
+        assert st.EXECUTING?; st := Jump(st);
+        assert st.EXECUTING?; st := block_0_0x0bdd(st);
         return st;
     }
 
-    method {:verify false} block_0_0x0bdd(st': EvmState.ExecutingState) returns (st'': EvmState.State)
+    method {:verify false} block_0_0x0bdd(st': EvmState.ExecutingState) returns (st'': EvmState.TerminatedState)
     requires st'.evm.code == Code.Create(BYTECODE_0)
     requires st'.WritesPermitted() && st'.PC() == 0x0bdd
     requires st'.Operands() == 4
     requires (st'.Peek(2) == 0x424)
+    requires Memory.Size(st'.evm.memory) >= 0x60 && st'.Read(0x40) == 0x80 // added by djp
+    //
+    ensures st''.RETURNS?
     {
+        ghost var sender := st'.Peek(1);
+        ghost var guy := st'.Peek(0);
         var st := st';
         st := JumpDest(st);
-        st := Push1(st,0x04);
+        // guy sender 0x424 ?
+        st := Push1(st,0x04); // slot number?
+        // 0x4 guy sender 0x424 ?
         st := Push1(st,0x20);
+        // 0x20 0x4 guy sender 0x424 ?
         st := MStore(st);
+        // guy sender 0x424 ? | mem[0x20:=0x4]
         st := Dup(st,2);
+        // sender guy sender 0x424 ? | mem[0x20:=0x4]
         st := Push1(st,0x00);
+        // 0x00 sender guy sender 0x424 ? | mem[0x20:=0x4]
         st := MStore(st);
+        // guy sender 0x424 ? | mem[0x00:=sender,0x20:=0x4]
+        assert st.Peek(2) == 0x424;
+        assert st.Operands() == 4;
         st := Push1(st,0x40);
+        // 0x40 guy sender 0x424 ? | mem[0x00:=sender,0x20:=0x4]
         st := Push1(st,0x00);
-        st := Keccak256(st);
+        // 0x00 0x40 guy sender 0x424 ? | mem[0x00:=sender,0x20:=0x4]
+        st := Keccak256(st); // 0x4; sender
+        // h1 guy sender 0x424 ? | mem[0x00:=sender,0x20:=0x4]
         st := Push1(st,0x20);
+        // 0x20 h guy sender 0x424 ? | mem[0x00:=sender,0x20:=0x4]
         st := MStore(st);
+        // guy sender 0x424 ? | mem[0x00:=sender,0x20:=h1]
         st := Dup(st,1);
+        // guy guy sender 0x424 ? | mem[0x00:=sender,0x20:=h1]
         st := Push1(st,0x00);
+        // 0x00 guy guy sender 0x424 ? | mem[0x00:=sender,0x20:=h1]
         st := MStore(st);
+        // guy sender 0x424 ? | mem[0x00:=guy,0x20:=h1]
+        assert st.Peek(2) == 0x424;
+        assert st.Operands() == 4;
         st := Push1(st,0x40);
+        // 0x40 guy sender 0x424 ? | mem[0x00:=guy,0x20:=h1]
         st := Push1(st,0x00);
+        // 0x00 0x40 guy sender 0x424 ? | mem[0x00:=guy,0x20:=h1]
         st := Keccak256(st);
+        // h2 guy sender 0x424 ? | mem[0x00:=guy,0x20:=h1]
         st := Push1(st,0x00);
+        // 0x00 h2 guy sender 0x424 ? | mem[0x00:=guy,0x20:=h1]
         st := Swap(st,2);
+        // guy h2 0x00 sender 0x424 ? | mem[0x00:=guy,0x20:=h1]
         st := Pop(st);
+        // h2 0x00 sender 0x424 ? | mem[0x00:=guy,0x20:=h1]
         st := Swap(st,2);
+        // sender 0x00 h2 0x424 ? | mem[0x00:=guy,0x20:=h1]
         st := Pop(st);
+        // 0x00 h2 0x424 ? | mem[0x00:=guy,0x20:=h1]
         st := Pop(st);
+        // h2 0x424 ? | mem[0x00:=guy,0x20:=h1]
         st := SLoad(st);
+        // wad 0x424 ? | mem[0x00:=guy,0x20:=h1]
         st := Dup(st,2);
+        // 0x424 wad 0x424 ? | mem[0x00:=guy,0x20:=h1]
         assume st.IsJumpDest(0x424);
         st := Jump(st);
+        // wad 0x424 ? | mem[0x00:=guy,0x20:=h1]
         st := block_0_0x0424(st);
         return st;
     }
 
-    method {:verify false} block_0_0x0424(st': EvmState.ExecutingState) returns (st'': EvmState.State)
+    method {:verify false} block_0_0x0424(st': EvmState.ExecutingState) returns (st'': EvmState.TerminatedState)
     requires st'.evm.code == Code.Create(BYTECODE_0)
     requires st'.WritesPermitted() && st'.PC() == 0x0424
     requires st'.Operands() == 3
     requires (st'.Peek(1) == 0x424)
+    requires Memory.Size(st'.evm.memory) >= 0x60 && st'.Read(0x40) == 0x80 // added by djp
+    //
+    ensures st''.RETURNS?
     {
         var st := st';
         st := JumpDest(st);
